PEano attempt1

theories/Logic/cut_elim.v
@@ -560,14 +560,12 @@ Proof.
   + destruct X as [[[[[[[X1 X2] X3] X4] X5] X6] X7] X8]. repeat split; simpl; auto.
     * rewrite w_rule_ptree_formula; auto. unfold w_rule_sub_formula. simpl. rewrite X1. rewrite formula_sub_ind_lor. simpl. rewrite eq_nat_refl. rewrite eq_f_refl. simpl. rewrite non_target_sub. auto. rewrite non_target_fit. auto.
     * apply w_rule_valid; auto. rewrite X1. simpl. rewrite non_target_fit. auto.
-    * rewrite w_rule_ptree_formula; auto. unfold w_rule_sub_formula. simpl. rewrite X3. simpl. rewrite eq_nat_refl. rewrite eq_f_refl. simpl. rewrite non_target_sub. auto. rewrite non_target_fit. auto.
-    * 
-    admit.
+    * rewrite w_rule_ptree_formula; auto. unfold w_rule_sub_formula. simpl. rewrite X3. simpl. admit. (* rewrite eq_nat_refl. rewrite eq_f_refl. simpl. rewrite non_target_sub. auto. rewrite non_target_fit. auto. *)
     * apply w_rule_valid; auto. rewrite X3. auto.
     * admit.
     * rewrite <- w_rule_ptree_deg; auto.
     * rewrite w_rule_ptree_ord; auto. admit.
-    * admit. 
+    * rewrite w_rule_ptree_ord; auto. 
 - simpl. destruct (ord_succ (ord_max o o0)) eqn:F. simpl. auto.
   destruct f.
   + case (correct_a a) eqn:H.
@@ -845,42 +843,39 @@ terminates, we now complete the reasoning for:
 'if A is provable, it has a Cut-free proof' *)
 (* *)
 
-Definition comp (alpha : ord) : Type := (forall (A : formula) (d : nat),
-provable A (S d) alpha -> provable A d (ord_2_exp alpha)).
-
-Definition comp' (alpha : ord) : Type := (forall (P : ptree) (A : formula) (d : nat),
+Definition cut_remove (alpha : ord) : Type := (forall (P : ptree) (A : formula) (d : nat),
 P_proves P A (S d) alpha -> provable A d (ord_2_exp alpha)).
 
 Lemma cut_elim_aux0 : forall (alpha : ord), nf alpha -> forall (P : ptree) (A : formula) (d : nat),
    P_proves P A (S d) alpha -> provable A d (ord_2_exp alpha).
 Proof.
-apply (transfinite_induction comp').
-- intros. unfold comp'. destruct x as [| alpha1 n alpha2]. intros. apply (cut_elim_ord_Zero P). auto. case (ord_eqb (cons Zero 0 Zero) (cons alpha1 n alpha2)) eqn:O.
+apply (transfinite_induction cut_remove).
+- intros. unfold cut_remove. destruct x as [| alpha1 n alpha2]. intros. apply (cut_elim_ord_Zero P). auto. case (ord_eqb (cons Zero 0 Zero) (cons alpha1 n alpha2)) eqn:O.
   intros. apply ord_eqb_eq in O. destruct O. apply (cut_elim_ord_one P). auto. assert (ord_lt (cons Zero 0 Zero) (cons alpha1 n alpha2)).
   { destruct (ord_semiconnex (cons Zero 0 Zero) (cons alpha1 n alpha2)) as [O1 | [O1 | O1]]. auto. inversion O1; inversion H1. destruct O1. inversion O. }
   intros P. induction P.
   + intros. destruct X0 as [[[X1 X2] X3] X4]. simpl in X3,X4. destruct X2 as [H1 H2]. apply IHP. unfold P_proves. repeat split; simpl; auto. lia.
-  + intros. destruct X0 as [[[X1 X2] X3] X4]. simpl in X1,X3,X4. destruct X4. destruct X2 as [[H1 H2] H3]. unfold comp' in X.
+  + intros. destruct X0 as [[[X1 X2] X3] X4]. simpl in X1,X3,X4. destruct X4. destruct X2 as [[H1 H2] H3]. unfold cut_remove in X.
     assert (P_proves P A (S d) (ptree_ord P)). { unfold P_proves. repeat split; simpl; auto. } destruct (X (ptree_ord P) (ptree_ord_nf _ H2) H1 P A d X0) as [P1 [[[HP1 HP2] HP3] HP4]].
     exists (ord_up (ord_2_exp o) P1). unfold P_proves. repeat split; simpl; auto. rewrite HP4. apply ord_2_exp_monot; auto. apply ptree_ord_nf. auto. apply nf_2_exp. auto.
   + intros. destruct X0 as [[[X1 X2] X3] X4]. simpl in X1,X3,X4. destruct X4. destruct d. exists (ord_up (ord_2_exp Zero) (node f)). unfold P_proves. repeat split; simpl; auto. apply zero_lt. apply single_nf. apply zero_nf.
     exists (ord_up (ord_2_exp Zero) (deg_up (S d) (node f))). unfold P_proves. repeat split; simpl; auto. apply zero_lt. lia. apply single_nf. apply zero_nf.
-  + intros. destruct X0 as [[[X1 X2] X3] X4]. simpl in X1,X3,X4. destruct X4. destruct X2 as [[[H1 H2] H3] H4]. unfold comp' in X.
+  + intros. destruct X0 as [[[X1 X2] X3] X4]. simpl in X1,X3,X4. destruct X4. destruct X2 as [[[H1 H2] H3] H4]. unfold cut_remove in X.
     assert (P_proves P (lor f f0) (S d) o). { unfold P_proves. repeat split; simpl; auto. lia. } pose (IHP _ _ X0). destruct p as [P1 [[[HP1 HP2] HP3] HP4]]. exists (exchange_ab f f0 (ptree_deg P1) (ptree_ord P1) P1). repeat split; simpl; auto.    
-  + intros. destruct X0 as [[[X1 X2] X3] X4]. simpl in X1,X3,X4. destruct X4. destruct X2 as [[[H1 H2] H3] H4]. unfold comp' in X.
+  + intros. destruct X0 as [[[X1 X2] X3] X4]. simpl in X1,X3,X4. destruct X4. destruct X2 as [[[H1 H2] H3] H4]. unfold cut_remove in X.
     assert (P_proves P (lor (lor f f0) f1) (S d) o). { unfold P_proves. repeat split; simpl; auto. lia. } pose (IHP _ _ X0). destruct p as [P1 [[[HP1 HP2] HP3] HP4]]. exists (exchange_cab f f0 f1 (ptree_deg P1) (ptree_ord P1) P1). repeat split; simpl; auto.
-  + intros. destruct X0 as [[[X1 X2] X3] X4]. simpl in X1,X3,X4. destruct X4. destruct X2 as [[[H1 H2] H3] H4]. unfold comp' in X.
+  + intros. destruct X0 as [[[X1 X2] X3] X4]. simpl in X1,X3,X4. destruct X4. destruct X2 as [[[H1 H2] H3] H4]. unfold cut_remove in X.
     assert (P_proves P (lor (lor f f0) f1) (S d) o). { unfold P_proves. repeat split; simpl; auto. lia. } pose (IHP _ _ X0). destruct p as [P1 [[[HP1 HP2] HP3] HP4]]. exists (exchange_abd f f0 f1 (ptree_deg P1) (ptree_ord P1) P1). repeat split; simpl; auto.    
-  + intros. destruct X0 as [[[X1 X2] X3] X4]. simpl in X1,X3,X4. destruct X4. destruct X2 as [[[H1 H2] H3] H4]. unfold comp' in X.
+  + intros. destruct X0 as [[[X1 X2] X3] X4]. simpl in X1,X3,X4. destruct X4. destruct X2 as [[[H1 H2] H3] H4]. unfold cut_remove in X.
     assert (P_proves P (lor (lor (lor f f0) f1) f2) (S d) o). { unfold P_proves. repeat split; simpl; auto. lia. } pose (IHP _ _ X0). destruct p as [P1 [[[HP1 HP2] HP3] HP4]]. exists (exchange_cabd f f0 f1 f2 (ptree_deg P1) (ptree_ord P1) P1). repeat split; simpl; auto.    
-  + intros. destruct X0 as [[[X1 X2] X3] X4]. simpl in X1,X3,X4. destruct X4. destruct X2 as [[[H1 H2] H3] H4]. unfold comp' in X.
+  + intros. destruct X0 as [[[X1 X2] X3] X4]. simpl in X1,X3,X4. destruct X4. destruct X2 as [[[H1 H2] H3] H4]. unfold cut_remove in X.
     assert (P_proves P (lor f f) (S d) o). { unfold P_proves. repeat split; simpl; auto. lia. } pose (IHP _ _ X0). destruct p as [P1 [[[HP1 HP2] HP3] HP4]]. exists (contraction_a f (ptree_deg P1) (ptree_ord P1) P1). repeat split; simpl; auto.    
-  + intros. destruct X0 as [[[X1 X2] X3] X4]. simpl in X1,X3,X4. destruct X4. destruct X2 as [[[H1 H2] H3] H4]. unfold comp' in X.
+  + intros. destruct X0 as [[[X1 X2] X3] X4]. simpl in X1,X3,X4. destruct X4. destruct X2 as [[[H1 H2] H3] H4]. unfold cut_remove in X.
     assert (P_proves P (lor (lor f f) f0) (S d) o). { unfold P_proves. repeat split; simpl; auto. lia. } pose (IHP _ _ X0). destruct p as [P1 [[[HP1 HP2] HP3] HP4]]. exists (contraction_ad f f0 (ptree_deg P1) (ptree_ord P1) P1). repeat split; simpl; auto.
-  + intros. destruct X0 as [[[X1 X2] X3] X4]. simpl in X1,X3,X4. destruct X4. destruct X2 as [[[[H1 H2] H3] H4] H5]. unfold comp' in X.
+  + intros. destruct X0 as [[[X1 X2] X3] X4]. simpl in X1,X3,X4. destruct X4. destruct X2 as [[[[H1 H2] H3] H4] H5]. unfold cut_remove in X.
     assert (P_proves P f0 (S d) o). { unfold P_proves. repeat split; simpl; auto. lia. } destruct (X _ (ord_nf_succ _ H) (ord_succ_monot _) _ _ _ X0) as [P1 [[[HP1 HP2] HP3] HP4]]. exists (ord_up (ord_2_exp (ord_succ o)) (weakening_ad f f0 (ptree_deg P1) (ptree_ord P1) P1)). repeat split; simpl; auto.
     rewrite HP4. apply ord_succ_lt_exp_succ. apply ord_nf_succ. auto. apply succ_gt_one_gt_zero. auto. apply nf_2_exp. auto.  
-  + intros. destruct X0 as [[[X1 X2] X3] X4]. simpl in X1,X3,X4. destruct X4. destruct X2 as [[[[[[[H1 H2] H3] H4] H5] H6] H7] H8]. unfold comp' in X. case (eq_nat (max n0 n1) (S d)) eqn:E.
+  + intros. destruct X0 as [[[X1 X2] X3] X4]. simpl in X1,X3,X4. destruct X4. destruct X2 as [[[[[[[H1 H2] H3] H4] H5] H6] H7] H8]. unfold cut_remove in X. case (eq_nat (max n0 n1) (S d)) eqn:E.
     * apply nat_eq_decid in E. case (lt_nat n0 n1) eqn:Y.
       --  rewrite (max_split1 _ _ Y) in E. symmetry in E. destruct E. assert (P_proves P2 (neg f0) (S d) o0). { unfold P_proves. repeat split; simpl; auto. lia. } assert (nf o0). rewrite H8. apply ptree_ord_nf. auto.
           destruct (X _ H9 (ord_max_succ_r _ _) _ _ _ X0) as [P7 [[[HP1 HP2] HP3] HP4]]. exists (ord_up (ord_2_exp (ord_succ (ord_max o o0))) (demorgan_ab f f0 n0 (ptree_deg P7) o (ord_2_exp o0) P1 P7)). repeat split; simpl; auto.
@@ -896,7 +891,7 @@ apply (transfinite_induction comp').
               exists (ord_up (ord_2_exp (ord_succ (ord_max o o0))) (demorgan_ab f f0 (ptree_deg P6) (ptree_deg P7) (ord_2_exp o) (ord_2_exp o0) P6 P7)). repeat split; simpl; auto.
               apply ord_max_exp_both; auto. apply nf_2_exp. auto. lia.
     * assert (d >= max n0 n1). { inversion X3. destruct H10. rewrite eq_nat_refl in E. inversion E. lia. } exists (ord_up (ord_2_exp (ord_succ (ord_max o o0))) (demorgan_ab f f0 n0 n1 o o0 P1 P2)). repeat split; simpl; auto. apply ord_succ_not_exp_fp. auto. apply nf_2_exp. auto.
-  + intros. destruct X0 as [[[X1 X2] X3] X4]. simpl in X1,X3,X4. destruct X4. destruct X2 as [[[[[[[H1 H2] H3] H4] H5] H6] H7] H8]. unfold comp' in X. case (eq_nat (max n0 n1) (S d)) eqn:E.
+  + intros. destruct X0 as [[[X1 X2] X3] X4]. simpl in X1,X3,X4. destruct X4. destruct X2 as [[[[[[[H1 H2] H3] H4] H5] H6] H7] H8]. unfold cut_remove in X. case (eq_nat (max n0 n1) (S d)) eqn:E.
     * apply nat_eq_decid in E. case (lt_nat n0 n1) eqn:Y.
       --  rewrite (max_split1 _ _ Y) in E. symmetry in E. destruct E. assert (P_proves P2 (lor (neg f0) f1) (S d) o0). { unfold P_proves. repeat split; simpl; auto. lia. } assert (nf o0). rewrite H8. apply ptree_ord_nf. auto.
           destruct (X _ H9 (ord_max_succ_r _ _) _ _ _ X0) as [P7 [[[HP1 HP2] HP3] HP4]]. exists (ord_up (ord_2_exp (ord_succ (ord_max o o0))) (demorgan_abd f f0 f1 n0 (ptree_deg P7) o (ord_2_exp o0) P1 P7)). repeat split; simpl; auto.
@@ -912,19 +907,19 @@ apply (transfinite_induction comp').
               exists (ord_up (ord_2_exp (ord_succ (ord_max o o0))) (demorgan_abd f f0 f1 (ptree_deg P6) (ptree_deg P7) (ord_2_exp o) (ord_2_exp o0) P6 P7)). repeat split; simpl; auto.
               apply ord_max_exp_both; auto. apply nf_2_exp. auto. lia.
     * assert (d >= max n0 n1). { inversion X3. destruct H10. rewrite eq_nat_refl in E. inversion E. lia. } exists (ord_up (ord_2_exp (ord_succ (ord_max o o0))) (demorgan_abd f f0 f1 n0 n1 o o0 P1 P2)). repeat split; simpl; auto. apply ord_succ_not_exp_fp. auto. apply nf_2_exp. auto.  
-  + intros. destruct X0 as [[[X1 X2] X3] X4]. simpl in X1,X3,X4. destruct X4. destruct X2 as [[[H1 H2] H3] H4]. unfold comp' in X.
+  + intros. destruct X0 as [[[X1 X2] X3] X4]. simpl in X1,X3,X4. destruct X4. destruct X2 as [[[H1 H2] H3] H4]. unfold cut_remove in X.
     assert (P_proves P f (S d) o). { unfold P_proves. repeat split; simpl; auto. lia. } destruct (X _ (ord_nf_succ _ H) (ord_succ_monot _) _ _ _ X0) as [P1 [[[HP1 HP2] HP3] HP4]]. exists (ord_up (ord_2_exp (ord_succ o)) (negation_a f (ptree_deg P1) (ptree_ord P1) P1)). repeat split; simpl; auto.
     rewrite HP4. apply ord_succ_lt_exp_succ. apply ord_nf_succ. auto. apply succ_gt_one_gt_zero. auto. apply nf_2_exp. auto. 
-  + intros. destruct X0 as [[[X1 X2] X3] X4]. simpl in X1,X3,X4. destruct X4. destruct X2 as [[[H1 H2] H3] H4]. unfold comp' in X.
+  + intros. destruct X0 as [[[X1 X2] X3] X4]. simpl in X1,X3,X4. destruct X4. destruct X2 as [[[H1 H2] H3] H4]. unfold cut_remove in X.
     assert (P_proves P (lor f f0) (S d) o). { unfold P_proves. repeat split; simpl; auto. lia. } destruct (X _ (ord_nf_succ _ H) (ord_succ_monot _) _ _ _ X0) as [P1 [[[HP1 HP2] HP3] HP4]]. exists (ord_up (ord_2_exp (ord_succ o)) (negation_ad f f0 (ptree_deg P1) (ptree_ord P1) P1)). repeat split; simpl; auto.
     rewrite HP4. apply ord_succ_lt_exp_succ. apply ord_nf_succ. auto. apply succ_gt_one_gt_zero. auto. apply nf_2_exp. auto. 
-  + intros. destruct X0 as [[[X1 X2] X3] X4]. simpl in X1,X3,X4. destruct X4. destruct X2 as [[[[H1 H2] H3] H4] H5]. unfold comp' in X.
+  + intros. destruct X0 as [[[X1 X2] X3] X4]. simpl in X1,X3,X4. destruct X4. destruct X2 as [[[[H1 H2] H3] H4] H5]. unfold cut_remove in X.
     assert (P_proves P (neg (substitution f n0 t)) (S d) o). { unfold P_proves. repeat split; simpl; auto. lia. } destruct (X _ (ord_nf_succ _ H) (ord_succ_monot _) _ _ _ X0) as [P1 [[[HP1 HP2] HP3] HP4]]. exists (ord_up (ord_2_exp (ord_succ o)) (quantification_a f n0 t (ptree_deg P1) (ptree_ord P1) P1)). repeat split; simpl; auto.
     rewrite HP4. apply ord_succ_lt_exp_succ. apply ord_nf_succ. auto. apply succ_gt_one_gt_zero. auto. apply nf_2_exp. auto. 
-  + intros. destruct X0 as [[[X1 X2] X3] X4]. simpl in X1,X3,X4. destruct X4. destruct X2 as [[[[H1 H2] H3] H4] H5]. unfold comp' in X.
+  + intros. destruct X0 as [[[X1 X2] X3] X4]. simpl in X1,X3,X4. destruct X4. destruct X2 as [[[[H1 H2] H3] H4] H5]. unfold cut_remove in X.
     assert (P_proves P (lor (neg (substitution f n0 t)) f0) (S d) o). { unfold P_proves. repeat split; simpl; auto. lia. } destruct (X _ (ord_nf_succ _ H) (ord_succ_monot _) _ _ _ X0) as [P1 [[[HP1 HP2] HP3] HP4]]. exists (ord_up (ord_2_exp (ord_succ o)) (quantification_ad f f0 n0 t (ptree_deg P1) (ptree_ord P1) P1)). repeat split; simpl; auto.
     rewrite HP4. apply ord_succ_lt_exp_succ. apply ord_nf_succ. auto. apply succ_gt_one_gt_zero. auto. apply nf_2_exp. auto. 
-  + intros. rename X0 into IHP. destruct X1 as [[[X1 X2] X3] X4]. simpl in X1,X3,X4. inversion X4. destruct H2,H3,H4. unfold comp' in X.
+  + intros. rename X0 into IHP. destruct X1 as [[[X1 X2] X3] X4]. simpl in X1,X3,X4. inversion X4. destruct H2,H3,H4. unfold cut_remove in X.
     unfold valid in X2. fold valid in X2. assert (forall m, P_proves (p m) (substitution f n0 (represent m)) (S d) o).
     { intros. unfold P_proves. destruct (X2 m) as [[[Y1 Y2] Y3] Y4]. repeat split; simpl; auto. destruct Y4. lia. }
     case (ord_eqb  (cons (ord_2_exp o) 0 Zero) (ord_2_exp (cons o 0 Zero))) eqn:X5.
@@ -955,7 +950,7 @@ apply (transfinite_induction comp').
           ++  destruct X as [P [[[HP1 HP2] HP3] HP4]]. simpl. auto.
           ++  destruct X as [P [[[HP1 HP2] HP3] HP4]]. simpl. auto.
           ++  apply single_nf. auto.
-  + intros. rename X0 into IHP. destruct X1 as [[[X1 X2] X3] X4]. simpl in X1,X3,X4. inversion X4. destruct H2,H3,H4. unfold comp' in X.
+  + intros. rename X0 into IHP. destruct X1 as [[[X1 X2] X3] X4]. simpl in X1,X3,X4. inversion X4. destruct H2,H3,H4. unfold cut_remove in X.
     unfold valid in X2. fold valid in X2. assert (forall m, P_proves (p m) (lor (substitution f n0 (represent m)) f0) (S d) o).
     { intros. unfold P_proves. destruct (X2 m) as [[[Y1 Y2] Y3] Y4]. repeat split; simpl; auto. destruct Y4. lia. }
     case (ord_eqb  (cons (ord_2_exp o) 0 Zero) (ord_2_exp (cons o 0 Zero))) eqn:X5.
@@ -1014,7 +1009,7 @@ apply (transfinite_induction comp').
                     { apply ord_ltb_lt. auto. }
                     { rewrite ord_succ_lt_exp_succ_dub_succ in Y2. inversion Y2. rewrite H7,H8. apply ord_max_nf; apply ptree_ord_nf; auto. apply ord_lt_ltb. apply ord_succ_not_exp_fp. rewrite Y1. auto. }
                     { apply ord_eqb_eq in Y2. destruct Y2. rewrite ord_eqb_refl in Y. inversion Y. } }
-                  { simpl. rewrite Y1. simpl. rewrite <- Y1. apply ord_succ_not_exp_fp. rewrite Y1. auto. }
+                  { unfold ptree_ord. rewrite <- Y1. rewrite (ord_max_lem2 _ _ (ltb_asymm _ _(ord_lt_ltb _ _ (ord_max_succ_r _ _)))). admit. (* pose ord_succ_lt_exp_succ_dub_succ. apply ord_succ_not_exp_fp. rewrite Y1. auto. *) }
               **  apply cut_elimination_valid; auto.
               **  apply nf_2_exp. auto.
               **  unfold ptree_deg. fold ptree_deg. unfold cut_elimination. unfold ptree_ord. rewrite Y1. destruct f0.
@@ -1023,10 +1018,10 @@ apply (transfinite_induction comp').
                     { simpl. lia. } }
                   { simpl. rewrite (nat_eq_decid _ _ E1) in X3. inversion X3. lia. simpl in H10. lia. }
                   { simpl. rewrite (nat_eq_decid _ _ E1) in X3. inversion X3. lia. simpl in H10. lia. }
-                  { admit. }
+                  { simpl in *. admit. }
 
     * assert ((S (num_conn f0)) < (max n0 n1)) as E2. apply nat_ne_symm in E1. rewrite (nat_eq_decid _ _ (nat_max_right_not _ _ E1)). apply (max_lem2 _ _ E1).
-      intros. destruct X0 as [[[X1 X2] X3] X4]. simpl in X1,X3,X4. destruct X4. destruct X2 as [[[[[[[H1 H2] H3] H4] H5] H6] H7] H8]. unfold comp' in X. case (eq_nat (max (max n0 n1) (S (num_conn f0))) (S d)) eqn:E.
+      intros. destruct X0 as [[[X1 X2] X3] X4]. simpl in X1,X3,X4. destruct X4. destruct X2 as [[[[[[[H1 H2] H3] H4] H5] H6] H7] H8]. unfold cut_remove in X. case (eq_nat (max (max n0 n1) (S (num_conn f0))) (S d)) eqn:E.
       --  assert ((S (num_conn f0)) < (max n0 n1)). apply nat_ne_symm in E1. rewrite (nat_eq_decid _ _ (nat_max_right_not _ _ E1)). apply (max_lem2 _ _ E1).
           apply nat_eq_decid in E. case (lt_nat n0 n1) eqn:Y.
           ++  rewrite (max_split1 _ _ Y) in E. symmetry in E. destruct E. assert (P_proves P2 (neg f0) (S d) o0). { unfold P_proves. repeat split; simpl; auto. lia. } assert (nf o0). rewrite H8. apply ptree_ord_nf. auto.
