theories/gentzen.v
@@ -13,6 +13,7 @@ From Systems Require Import fol.
 From Systems Require Import PA_omega.
 From Systems Require Import proof_trees.
 From Systems Require Import substitute.
+From Systems Require Import cut_elim.
 Notation "b1 && b2" := (andb b1 b2).
 Notation "b1 || b2" := (orb b1 b2).
 Notation eq_nat := Nat.eqb.
@@ -85,152 +86,29 @@ intros P. induction P.
 - intros. destruct X as [[[HP1 HP2] HP3] HP4]. simpl in HP1,HP3,HP4. destruct HP2 as [[[[[[[HP2a HP2b] HP2c] HP2d] HP2e] HP2f] HP2g] HP2h]. lia.
 Qed.
 
-
-Lemma cut_elim_aux1 : forall (alpha : ord) (P : ptree) (A : formula) (d : nat), P_proves P A (S d) alpha -> provable A d (ord_2_exp alpha).
-Proof.
-intros. inversion X. destruct X0 as [[H1 H2] H3]. pose (ptree_ord_nf _ H2). destruct H. admit.
-Admitted.
-
-Lemma cut_elim_aux2 : forall (A : formula) (d : nat),
-  {alpha : ord & provable A d alpha} -> {beta : ord & provable A 0 beta}.
-Proof.
-intros. induction d.
-- destruct X as [alpha H]. exists alpha. auto.
-- apply IHd. destruct X as [alpha H]. exists (ord_2_exp alpha). destruct H as [P H]. apply (cut_elim_aux1 _ _ _ _ H).
-Qed.
-
-Lemma cut_elim_aux3 : forall (A : formula) (d : nat) (alpha : ord),
-  provable A d alpha -> {beta : ord & provable A 0 beta}.
-Proof. intros. apply (cut_elim_aux2 A d). exists alpha. auto. Qed.
-
-Fixpoint cut_free (P : ptree) : Type :=
-match P with
-| deg_up d P' => cut_free P'
-
-| ord_up alpha P' => cut_free P'
-
-| node A => True
-
-
-| exchange_ab A B d alpha P' => cut_free P'
-
-| exchange_cab C0 A B d alpha P' => cut_free P'
-
-| exchange_abd A B D d alpha P' => cut_free P'
-
-| exchange_cabd C0 A B D d alpha P' => cut_free P'
-
-| contraction_a A d alpha P' => cut_free P'
-
-| contraction_ad A D d alpha P' => cut_free P'
-
-
-| weakening_ad A D d alpha P' => cut_free P'
-
-| demorgan_ab A B d1 d2 alpha1 alpha2 P1 P2 => (cut_free P1) * (cut_free P2)
-
-| demorgan_abd A B D d1 d2 alpha1 alpha2 P1 P2 => (cut_free P1) * (cut_free P2)
-
-| negation_a A d alpha P' => cut_free P'
-
-| negation_ad A D d alpha P' => cut_free P'
-
-
-| quantification_a A n t d alpha P' => cut_free P'
-
-| quantification_ad A D n t d alpha P' => cut_free P'
-
-| w_rule_a A n d alpha g => forall (m : nat), cut_free (g m)
-
-| w_rule_ad A D n d alpha g => forall (m : nat), cut_free (g m)
-
-
-| cut_ca C0 A d1 d2 alpha1 alpha2 P1 P2 => False
-
-| cut_ad A D d1 d2 alpha1 alpha2 P1 P2 => False
-
-| cut_cad C0 A D d1 d2 alpha1 alpha2 P1 P2 => False
-
-end.
-
-
-Lemma cut_elim_aux4 : forall (P : ptree),
-  valid P -> ptree_deg P = 0 -> cut_free P.
-Proof.
-intros. induction P; simpl; auto.
-- destruct X as [H1 H2]. simpl in H. rewrite H in H1. lia.
-- destruct X as [[H1 H2] H3]. simpl in H. apply IHP; auto.
-- destruct X as [[[H1 H2] H3] H4]. simpl in H. rewrite H in H3.
-  apply IHP; auto.
-- destruct X as [[[H1 H2] H3] H4]. simpl in H. rewrite H in H3.
-  apply IHP; auto.
-- destruct X as [[[H1 H2] H3] H4]. simpl in H. rewrite H in H3.
-  apply IHP; auto.
-- destruct X as [[[H1 H2] H3] H4]. simpl in H. rewrite H in H3.
-  apply IHP; auto.
-- destruct X as [[[H1 H2] H3] H4]. simpl in H. rewrite H in H3.
-  apply IHP; auto.
-- destruct X as [[[H1 H2] H3] H4]. simpl in H. rewrite H in H3.
-  apply IHP; auto.
-- destruct X as [[[H1 H2] H3] H4]. simpl in H. rewrite H in H3.
-  apply IHP; auto.
-- destruct X as [[[[[[[H1 H2] H3] H4] H5] H6] H7] H8].
-  simpl in H. rewrite H5 in H. rewrite H6 in H.
-  destruct (max_0 _ _ H). split.
-  + apply IHP1; auto.
-  + apply IHP2; auto.
-- destruct X as [[[[[[[H1 H2] H3] H4] H5] H6] H7] H8].
-  simpl in H. rewrite H5 in H. rewrite H6 in H.
-  destruct (max_0 _ _ H). split.
-  + apply IHP1; auto.
-  + apply IHP2; auto.
-- destruct X as [[[H1 H2] H3] H4]. simpl in H. rewrite H in H3.
-  apply IHP; auto.
-- destruct X as [[[H1 H2] H3] H4]. simpl in H. rewrite H in H3.
-  apply IHP; auto.
-- destruct X as [[[H1 H2] H3] H4]. simpl in H. rewrite H in H3.
-  apply IHP; auto.
-- destruct X as [[[H1 H2] H3] H4]. simpl in H. rewrite H in H3.
-  apply IHP; auto.
-- rename f into A. rename p into g. rename n0 into d. rename o into alpha.
-  intros. simpl in H. simpl in X. destruct (X m) as [[[H1 H2] H3] H4].
-  rewrite H in H3. apply X0; auto. lia.
-- rename f into A. rename f0 into D. rename p into g.
-  rename n0 into d. rename o into alpha.
-  intros. simpl in H. simpl in X. destruct (X m) as [[[H1 H2] H3] H4].
-  rewrite H in H3. apply X0; auto. lia.
-- simpl in H. apply max_succ_0 in H. auto.
-- simpl in H. apply max_succ_0 in H. auto.
-- simpl in H. apply max_succ_0 in H. auto.
-Qed.
-
-Definition P_proves' (P : ptree) (A : formula) : Type :=
-  (ptree_formula P = A) * (valid P) *
-  {d : nat & ptree_deg P = d & {alpha : ord & ptree_ord P = alpha}}.
-
-Lemma cut_elim_aux5 : forall (A : formula) (d : nat) (alpha : ord),
-  provable A d alpha -> {P : ptree & P_proves' P A & cut_free P}.
-Proof.
-intros. apply cut_elim_aux3 in X. destruct X as [gamma [P [[[H1 H2] H3] H4]]].
-exists P.
-- unfold P_proves'. repeat split; auto.
-  exists 0; auto. lia. exists gamma; auto.
-- apply cut_elim_aux4; auto. lia.
-Qed.
-
 Lemma provable_not_danger : forall A d alpha, provable A d alpha -> dangerous_disjunct A = false.
 Proof.
 intros. case (dangerous_disjunct A) eqn:Y; auto.
 - destruct (cut_elim_aux3 _ _ _ X) as [beta [P HP]]. pose (danger_not_deg_0 P A 0 beta HP Y). inversion l.
 Qed.
 
-Lemma danger_not_provable : forall A P, dangerous_disjunct A = true -> valid P -> eq_f (ptree_formula P) A = false.
+Lemma danger_not_provable' : forall A P, dangerous_disjunct A = true -> valid P -> eq_f (ptree_formula P) A = false.
 Proof.
 intros. case (eq_f (ptree_formula P) A) eqn:Y; auto. intros. assert (provable (ptree_formula P) (ptree_deg P) (ptree_ord P)) as HP. exists P. repeat split; simpl; auto.
 pose (provable_not_danger _ _ _ HP). apply f_eq_decid in Y. destruct Y. rewrite H in e. inversion e.
 Qed.
 
-Lemma danger_not_theorem : forall A n alpha, PA_omega_theorem A n alpha -> dangerous_disjunct A = false.
+Lemma danger_not_provable : forall A, dangerous_disjunct A = true -> forall P d alpha, P_proves P A d alpha -> False.
+Proof.
+intros. destruct X as [[[X1 X2] X3] X4]. pose proof (danger_not_provable' _ _ H X2). destruct X1. rewrite eq_f_refl in H0. inversion H0.
+Qed.
+
+Lemma theorem_not_danger : forall A n alpha, PA_omega_theorem A n alpha -> dangerous_disjunct A = false.
 Proof.
 intros. apply (provable_not_danger _ _ _ (provable_theorem _ _ _ H)). 
+Qed.
+
+Lemma danger_not_theorem : forall A, dangerous_disjunct A = true -> forall n alpha, PA_omega_theorem A n alpha -> False.
+Proof.
+intros. apply (danger_not_provable _ H _ _ _ (projT2(provable_theorem _ _ _ H0))). 
 Qed.
